src/base/assert.v
@@ -1,0 +1,25 @@
+From iris.proofmode Require Import proofmode.
+From iris.program_logic Require Export weakestpre.
+
+From self.lang Require Import lang.
+From self.base Require Import proofmode.
+
+From iris.prelude Require Import options.
+
+Section lifting.
+  Context `{!nvmBaseFixedG Σ, nvmBaseDeltaG Σ}.
+
+  Lemma wp_assert E (Φ : thread_val → iProp Σ) e TV :
+    WP ThreadState e TV @ E {{ v, ⌜val_val v = #true⌝ ∧ ▷ Φ (ThreadVal #() (val_view v)) }} -∗
+    WP ThreadState (assert: e)%V TV @ E {{ Φ }}.
+  Proof.
+    iIntros "HΦ".
+    wp_lam.
+    wp_smart_apply (wp_wand with "HΦ"). iIntros ([v ?]) "[% ?]".
+    rewrite /thread_fill_item.
+    simpl in *.
+    subst.
+    wp_if.
+    done.
+  Qed.
+End lifting.
